template-coq/src/g_template_coq.ml
@@ -4,6 +4,7 @@ let _ = Mltop.add_known_module __coq_plugin_name
 # 6 "src/g_template_coq.mlg"
  
 
+open Attributes
 open Ltac_plugin
 open Names
 
@@ -13,13 +14,14 @@ let ltac_lcall tac args =
   let (location, name) = Loc.tag (Names.Id.of_string tac)
     (* Loc.tag @@ Names.Id.of_string tac *)
   in
-  Tacexpr.TacArg(Loc.tag @@ Tacexpr.TacCall
-                              (Loc.tag (Locus.ArgVar (CAst.make ?loc:location name),args)))
+  Tacexpr.TacArg(CAst.make ?loc:location (Tacexpr.TacCall
+                              (CAst.make (Locus.ArgVar (CAst.make ?loc:location name),args))))
 
 open Tacexpr
 open Tacinterp
 open Stdarg
 open Tacarg
+open Genredexpr
 
 let _ = Goptions.declare_bool_option {
   Goptions.optdepr = false;
@@ -45,9 +47,13 @@ let ltac_apply (f : Value.t) (args: Tacinterp.Value.t list) =
 let to_ltac_val c = Tacinterp.Value.of_constr c
 
 
-let run_template_program env evm pgm =
-  Run_template_monad.run_template_program_rec (fun _ -> ()) env (evm, pgm)
+let run_template_program env evm ~poly pgm =
+  Run_template_monad.run_template_program_rec ~poly (fun _ -> ()) env (evm, pgm)
 
+let fresh_env () = 
+  let env = Global.env () in
+  let sigma = Evd.from_env env in
+  env, sigma
 
 
 let () = Vernacextend.vernac_extend ~command:"TemplateCoq_Test_Quote" ~classifier:(fun _ -> Vernacextend.classify_as_query) ?entry:None 
@@ -55,19 +61,19 @@ let () = Vernacextend.vernac_extend ~command:"TemplateCoq_Test_Quote" ~classifie
                                      Vernacextend.TyTerminal ("Quote", 
                                      Vernacextend.TyNonTerminal (Extend.TUentry (Genarg.get_arg_tag wit_constr), 
                                      Vernacextend.TyNil))), (let coqpp_body def
-                                                            () ~st = 
+                                                            poly ~st = 
                                                             let () = 
                                                             
-# 58 "src/g_template_coq.mlg"
-        let (evm,env) = Pfedit.get_current_context () in
+# 64 "src/g_template_coq.mlg"
+        let (env, evm) = fresh_env () in
         let (evm, def) = Constrintern.interp_open_constr env evm def in
         let (evm, pgm) = EConstr.fresh_global env evm (Lazy.force Template_monad.ptmTestQuote) in
         let pgm = Constr.mkApp (EConstr.to_constr evm pgm, [|Constr.mkRel 0; EConstr.to_constr evm def|]) in
-        run_template_program env evm pgm 
+        run_template_program env evm ~poly pgm 
                                                              in st in fun def
                                                             ~atts ~st
                                                             -> coqpp_body def
-                                                            (Attributes.unsupported_attributes atts) ~st), None))]
+                                                            (Attributes.parse polymorphic atts) ~st), None))]
 
 let () = Vernacextend.vernac_extend ~command:"TemplateCoq_Quote_Definition" ~classifier:(fun _ -> Vernacextend.classify_as_sideeff) ?entry:None 
          [(Vernacextend.TyML (false, Vernacextend.TyTerminal ("Quote", 
@@ -76,16 +82,16 @@ let () = Vernacextend.vernac_extend ~command:"TemplateCoq_Quote_Definition" ~cla
                                      Vernacextend.TyTerminal (":=", Vernacextend.TyNonTerminal (
                                                                     Extend.TUentry (Genarg.get_arg_tag wit_constr), 
                                                                     Vernacextend.TyNil))))), 
-         (let coqpp_body name def () ~st = let () = 
-# 67 "src/g_template_coq.mlg"
-        let (evm,env) = Pfedit.get_current_context () in
+         (let coqpp_body name def poly ~st = let () = 
+# 73 "src/g_template_coq.mlg"
+        let (env, evm) = fresh_env () in
         let (evm, def) = Constrintern.interp_open_constr env evm def in
         let (evm, pgm) = EConstr.fresh_global env evm (Lazy.force Template_monad.ptmQuoteDefinition) in
         let pgm = Constr.mkApp (EConstr.to_constr evm pgm, [|Constr_quoter.TemplateCoqQuoter.quote_ident name; Constr.mkRel 0; EConstr.to_constr evm def|]) in
-        run_template_program env evm pgm 
-                                            in st in fun name
+        run_template_program env evm ~poly pgm 
+                                              in st in fun name
          def ~atts ~st -> coqpp_body name def
-         (Attributes.unsupported_attributes atts) ~st), None))]
+         (Attributes.parse polymorphic atts) ~st), None))]
 
 let () = Vernacextend.vernac_extend ~command:"TemplateCoq_Quote_Definition_Eval" ~classifier:(fun _ -> Vernacextend.classify_as_sideeff) ?entry:None 
          [(Vernacextend.TyML (false, Vernacextend.TyTerminal ("Quote", 
@@ -98,19 +104,19 @@ let () = Vernacextend.vernac_extend ~command:"TemplateCoq_Quote_Definition_Eval"
                                                                     Vernacextend.TyNonTerminal (
                                                                     Extend.TUentry (Genarg.get_arg_tag wit_constr), 
                                                                     Vernacextend.TyNil)))))))), 
-         (let coqpp_body name rd def () ~st = let () = 
-# 76 "src/g_template_coq.mlg"
-        let (evm, env) = Pfedit.get_current_context () in
+         (let coqpp_body name rd def poly ~st = let () = 
+# 82 "src/g_template_coq.mlg"
+        let (env, evm) = fresh_env () in
         let (evm, def) = Constrintern.interp_open_constr env evm def in
         (* TODO : implem quoting of tactic reductions so that we can use ptmQuoteDefinitionRed *)
         let (evm, rd) = Tacinterp.interp_redexp env evm rd in
-	let (evm, def) = Quoter.reduce env evm rd (EConstr.to_constr evm def) in
+	      let (evm, def) = Quoter.reduce env evm rd (EConstr.to_constr evm def) in
         let (evm, pgm) = EConstr.fresh_global env evm (Lazy.force Template_monad.ptmQuoteDefinition) in
         let pgm = Constr.mkApp (EConstr.to_constr evm pgm, [|Constr_quoter.TemplateCoqQuoter.quote_ident name; Constr.mkRel 0; def|]) in
-        run_template_program env evm pgm 
-                                               in st in fun name
+        run_template_program env evm ~poly pgm 
+                                                 in st in fun name
          rd def ~atts ~st -> coqpp_body name rd def
-         (Attributes.unsupported_attributes atts) ~st), None))]
+         (Attributes.parse polymorphic atts) ~st), None))]
 
 let () = Vernacextend.vernac_extend ~command:"TemplateCoq_Quote_Recursively_Definition" ~classifier:(fun _ -> Vernacextend.classify_as_sideeff) ?entry:None 
          [(Vernacextend.TyML (false, Vernacextend.TyTerminal ("Quote", 
@@ -120,16 +126,16 @@ let () = Vernacextend.vernac_extend ~command:"TemplateCoq_Quote_Recursively_Defi
                                      Vernacextend.TyTerminal (":=", Vernacextend.TyNonTerminal (
                                                                     Extend.TUentry (Genarg.get_arg_tag wit_constr), 
                                                                     Vernacextend.TyNil)))))), 
-         (let coqpp_body name def () ~st = let () = 
-# 88 "src/g_template_coq.mlg"
-        let (evm,env) = Pfedit.get_current_context () in
+         (let coqpp_body name def poly ~st = let () = 
+# 94 "src/g_template_coq.mlg"
+        let (env, evm) = fresh_env () in
         let (evm, def) = Constrintern.interp_open_constr env evm def in
         let (evm, pgm) = EConstr.fresh_global env evm (Lazy.force Template_monad.ptmQuoteRecDefinition) in
         let pgm = Constr.mkApp (EConstr.to_constr evm pgm, [|Constr_quoter.TemplateCoqQuoter.quote_ident name; Constr.mkRel 0; EConstr.to_constr evm def|]) in
-        run_template_program env evm pgm 
-                                            in st in fun name
+        run_template_program env evm ~poly pgm 
+                                              in st in fun name
          def ~atts ~st -> coqpp_body name def
-         (Attributes.unsupported_attributes atts) ~st), None))]
+         (Attributes.parse polymorphic atts) ~st), None))]
 
 let () = Vernacextend.vernac_extend ~command:"TemplateCoq_Make_Definition" ~classifier:(fun _ -> Vernacextend.classify_as_sideeff) ?entry:None 
          [(Vernacextend.TyML (false, Vernacextend.TyTerminal ("Make", 
@@ -138,53 +144,53 @@ let () = Vernacextend.vernac_extend ~command:"TemplateCoq_Make_Definition" ~clas
                                      Vernacextend.TyTerminal (":=", Vernacextend.TyNonTerminal (
                                                                     Extend.TUentry (Genarg.get_arg_tag wit_constr), 
                                                                     Vernacextend.TyNil))))), 
-         (let coqpp_body name def () ~st = let () = 
-# 97 "src/g_template_coq.mlg"
-        let (evm, env) = Pfedit.get_current_context () in
+         (let coqpp_body name def poly ~st = let () = 
+# 103 "src/g_template_coq.mlg"
+        let (env, evm) = fresh_env () in
         let (evm, def) = Constrintern.interp_open_constr env evm def in
         let (evm, pgm) = EConstr.fresh_global env evm (Lazy.force Template_monad.ptmMkDefinition) in
         let pgm = Constr.mkApp (EConstr.to_constr evm pgm, [|Constr_quoter.TemplateCoqQuoter.quote_ident name; EConstr.to_constr evm def|]) in
-        run_template_program env evm pgm 
-                                            in st in fun name
+        run_template_program env evm ~poly pgm 
+                                              in st in fun name
          def ~atts ~st -> coqpp_body name def
-         (Attributes.unsupported_attributes atts) ~st), None))]
+         (Attributes.parse polymorphic atts) ~st), None))]
 
 let () = Vernacextend.vernac_extend ~command:"TemplateCoq_Make_Inductive" ~classifier:(fun _ -> Vernacextend.classify_as_sideeff) ?entry:None 
          [(Vernacextend.TyML (false, Vernacextend.TyTerminal ("Make", 
                                      Vernacextend.TyTerminal ("Inductive", 
                                      Vernacextend.TyNonTerminal (Extend.TUentry (Genarg.get_arg_tag wit_constr), 
                                      Vernacextend.TyNil))), (let coqpp_body def
-                                                            () ~st = 
+                                                            poly ~st = 
                                                             let () = 
                                                             
-# 106 "src/g_template_coq.mlg"
-        let (evm, env) = Pfedit.get_current_context () in
+# 112 "src/g_template_coq.mlg"
+        let (env, evm) = fresh_env () in
         let (evm, def) = Constrintern.interp_open_constr env evm def in
         let (evm, pgm) = EConstr.fresh_global env evm (Lazy.force Template_monad.ptmMkInductive) in
         let pgm = Constr.mkApp (EConstr.to_constr evm pgm, [|EConstr.to_constr evm def|]) in
-        run_template_program env evm pgm 
+        run_template_program env evm ~poly pgm 
                                                              in st in fun def
                                                             ~atts ~st
                                                             -> coqpp_body def
-                                                            (Attributes.unsupported_attributes atts) ~st), None))]
+                                                            (Attributes.parse polymorphic atts) ~st), None))]
 
 let () = Vernacextend.vernac_extend ~command:"TemplateCoq_Run_Template_Program" ~classifier:(fun _ -> Vernacextend.classify_as_sideeff) ?entry:None 
          [(Vernacextend.TyML (false, Vernacextend.TyTerminal ("Run", 
                                      Vernacextend.TyTerminal ("TemplateProgram", 
                                      Vernacextend.TyNonTerminal (Extend.TUentry (Genarg.get_arg_tag wit_constr), 
                                      Vernacextend.TyNil))), (let coqpp_body def
-                                                            () ~st = 
+                                                            poly ~st = 
                                                             let () = 
                                                             
-# 115 "src/g_template_coq.mlg"
-        let (evm, env) = Pfedit.get_current_context () in
+# 121 "src/g_template_coq.mlg"
+        let (env, evm) = fresh_env () in
         let (evm, def) = Constrintern.interp_open_constr env evm def in
         let pgm = EConstr.to_constr evm def in
-        run_template_program env evm pgm 
+        run_template_program env evm ~poly pgm 
                                                              in st in fun def
                                                             ~atts ~st
                                                             -> coqpp_body def
-                                                            (Attributes.unsupported_attributes atts) ~st), None))]
+                                                            (Attributes.parse polymorphic atts) ~st), None))]
 
 let () = Tacentries.tactic_extend __coq_plugin_name "TemplateCoq_quote_term" ~level:0 
          [(Tacentries.TyML (Tacentries.TyIdent ("quote_term", Tacentries.TyArg (
@@ -193,9 +199,9 @@ let () = Tacentries.tactic_extend __coq_plugin_name "TemplateCoq_quote_term" ~le
                                                               Extend.TUentry (Genarg.get_arg_tag wit_tactic), 
                                                               Tacentries.TyNil))), 
            (fun c tac ist -> 
-# 126 "src/g_template_coq.mlg"
-        (** quote the given term, pass the result to t **)
-        Proofview.Goal.nf_enter begin fun gl ->
+# 132 "src/g_template_coq.mlg"
+        (* quote the given term, pass the result to t *)
+        Proofview.Goal.enter begin fun gl ->
           let env = Proofview.Goal.env gl in
           let c = EConstr.to_constr (Proofview.Goal.sigma gl) c in
 	  let c = Constr_quoter.TermReify.quote_term env c in
@@ -210,7 +216,7 @@ let () = Tacentries.tactic_extend __coq_plugin_name "TemplateCoq_denote_term" ~l
                                                                Extend.TUentry (Genarg.get_arg_tag wit_tactic), 
                                                                Tacentries.TyNil))), 
            (fun c tac ist -> 
-# 137 "src/g_template_coq.mlg"
+# 143 "src/g_template_coq.mlg"
         Proofview.Goal.enter (begin fun gl ->
          let evm = Proofview.Goal.sigma gl in
          let evm, c = Constr_denoter.denote_term evm (EConstr.to_constr evm c) in
@@ -224,12 +230,14 @@ let () = Tacentries.tactic_extend __coq_plugin_name "TemplateCoq_run_template_pr
                             Tacentries.TyArg (Extend.TUentry (Genarg.get_arg_tag wit_constr), 
                             Tacentries.TyArg (Extend.TUentry (Genarg.get_arg_tag wit_tactic), 
                             Tacentries.TyNil))), (fun c tac ist -> 
-# 147 "src/g_template_coq.mlg"
-        roofview.Goal.enter (begin fun gl ->
+# 153 "src/g_template_coq.mlg"
+        let open Proofview.Notations in
+        Proofview.tclProofInfo [@ocaml.warning "-3"] >>= fun (name, poly) ->
+        Proofview.Goal.enter (begin fun gl ->
          let env = Proofview.Goal.env gl in
          let evm = Proofview.Goal.sigma gl in
          let ret = ref None in
-         Run_template_monad.run_template_program_rec ~intactic:true (fun x -> ret := Some x) env (evm, EConstr.to_constr evm c);
+         Run_template_monad.run_template_program_rec ~poly ~intactic:true (fun x -> ret := Some x) env (evm, EConstr.to_constr evm c);
          match !ret with
            Some (env, evm, t) ->
             Proofview.tclTHEN
