template-coq/src/quoted.ml
@@ -42,13 +42,13 @@ let list_to_string l =
 
 (* Remove '#' from names *)
 let clean_name s =
-  let l = List.rev (CString.split '#' s) in
+  let l = List.rev (CString.split_on_char '#' s) in
   match l with
     s :: rst -> s
   | [] -> raise (Failure "Empty name cannot be quoted")
 
 let split_name s : (Names.DirPath.t * Names.Id.t) =
-  let ss = List.rev (CString.split '.' s) in
+  let ss = List.rev (CString.split_on_char '.' s) in
   match ss with
     nm :: rst ->
      let nm = clean_name nm in
