template-coq/src/run_template_monad.mli
@@ -1,6 +1,7 @@
 val declare_inductive : Environ.env -> Evd.evar_map -> Constr.t -> unit
 
 val run_template_program_rec :
-           ?intactic:bool ->
-           (Environ.env * Evd.evar_map * Constr.t -> unit) ->
-           Environ.env -> Evd.evar_map * Constr.t -> unit
+    poly:bool ->
+    ?intactic:bool ->
+    (Environ.env * Evd.evar_map * Constr.t -> unit) ->
+    Environ.env -> Evd.evar_map * Constr.t -> unit
