template-coq/theories/AstUtils.v
@@ -318,28 +318,23 @@ Fixpoint lookup_mind_decl (id : ident) (decls : global_env)
     | _ :: tl => lookup_mind_decl id tl
     end.
 
+Definition universes_entry_of_decl (u : universes_decl) : universes_entry :=
+  match u with
+  | Polymorphic_ctx ctx => Polymorphic_entry (map nNamed (fst ctx)) (Universes.AUContext.repr ctx)
+  | Monomorphic_ctx ctx => Monomorphic_entry ctx
+  end.
+
 (* was mind_decl_to_entry *)
 Definition mind_body_to_entry (decl : mutual_inductive_body)
   : mutual_inductive_entry.
 Proof.
   refine {| mind_entry_record := None; (* not a record *)
             mind_entry_finite := Finite; (* inductive *)
-            mind_entry_params := _;
+            mind_entry_params := decl.(ind_params);
             mind_entry_inds := _;
-            mind_entry_universes := decl.(ind_universes);
+            mind_entry_universes := universes_entry_of_decl decl.(ind_universes);
             mind_entry_variance := decl.(ind_variance);
             mind_entry_private := None |}.
-  - refine (match List.hd_error decl.(ind_bodies) with
-            | Some i0 => List.rev _
-            | None => nil (* assert false: at least one inductive in a mutual block *)
-            end).
-    pose (typ := decompose_prod i0.(ind_type)).
-    destruct typ as [[names types] _].
-    apply (List.firstn decl.(ind_npars)) in names.
-    apply (List.firstn decl.(ind_npars)) in types.
-    refine (List.combine _ _).
-    exact (List.map get_ident names).
-    exact (List.map LocalAssum types).
   - refine (List.map _ decl.(ind_bodies)).
     intros [].
     refine {| mind_entry_typename := ind_name;
